theories/example.v
@@ -38,28 +38,6 @@ Definition trc_add_x1_x2_x3 : trc :=
   WriteReg "R1" [] (Val_Symbolic 3452) Mk_annot
 ].
 
-(* Lemma add_x1_x2_x3_trace n2 n3 : *)
-(*   trc_add_x1_x2_x3 ~{ trace_module, [ *)
-(*                     Vis (LReadReg "R2" [] (Val_Bits [BV{64} n2])); *)
-(*                     Vis (LReadReg "R3" [] (Val_Bits [BV{64} n3])); *)
-(*                     Vis (LWriteReg "R1" [] (Val_Bits (bv_extract 63 0 (bv_add (bv_zero_extend 64 [BV{64} n2]) (bv_zero_extend 64 [BV{64} n3]))))) *)
-(*                 ] }~> []. *)
-(* Proof. *)
-(*   do_trace_step. *)
-(*   do_trace_step. *)
-(*   do_trace_step. *)
-(*   do_trace_step. *)
-(*   do_trace_step. *)
-(*   do_trace_step. *)
-(*   do_trace_step. *)
-(*   do_trace_step. *)
-(*   do_trace_step. *)
-(*   do_trace_step. *)
-(*   do_trace_step. *)
-(*   do_trace_step. *)
-(*   by apply: TraceEnd. *)
-(* Qed. *)
-
 (*
 C:
 int test() {
@@ -170,50 +148,8 @@ Definition test_state_global := {|
     seq_mem := ∅
 |}.
 
-(* Ltac do_seq_step := *)
-(*   apply: (TraceStep' _ _ seq_module (_, _)); [ econstructor; [done|solve_trace_step| try left; done] | done |]; simpl. *)
-
-(* Ltac do_seq_step_jmp := *)
-(*   apply: (TraceStep' _ _ seq_module (_, _)); [ econstructor; [done|solve_trace_step| ]; *)
-(*                        eexists _, _; repeat (split; first done); vm_compute; split => //; left | done |]; simpl. *)
-
-(* Lemma test_state_trace : *)
-(*   (test_state_global, test_state_local) ~{ seq_module, [Vis (SWriteReg "OUT" [] (Val_Bits [BV{64} 0x0])) ] }~> -. *)
-(* Proof. *)
-(*   eexists _. *)
-(*   do_seq_step_jmp. *)
-(*   do_seq_step. *)
-(*   do_seq_step. *)
-(*   do_seq_step. *)
-(*   do_seq_step. *)
-(*   do_seq_step. *)
-(*   do_seq_step. *)
-(*   do_seq_step_jmp. *)
-(*   do_seq_step. *)
-(*   do_seq_step_jmp. *)
-(*   do_seq_step. *)
-(*   do_seq_step. *)
-(*   do_seq_step. *)
-(*   do_seq_step. *)
-(*   do_seq_step. *)
-(*   do_seq_step. *)
-(*   do_seq_step. *)
-(*   do_seq_step. *)
-(*   do_seq_step. *)
-(*   do_seq_step_jmp. *)
-(*   do_seq_step. *)
-(*   do_seq_step. *)
-(*   do_seq_step. *)
-(*   do_seq_step. *)
-(*   do_seq_step. *)
-(*   apply: TraceEnd. *)
-(* Qed. *)
 
 Definition test_state_spec : list seq_label := [ SInstrTrap ([BV{64} 0x0000000010300008]) ].
-
-Global Instance simpl_normalize_valu_end v1 v2:
-  SimplAndUnsafe true (normalize_valu v1 v2) (λ T, v1 = v2 ∧ T) | 1000.
-Proof. move => ?. done. Qed.
 
 Lemma test_state_iris `{!islaG Σ} `{!threadG} :
   instr 0x0000000010300000 (Some [trc_bl_0x100]) -∗
@@ -496,25 +432,22 @@ Definition trc_b_0x8 : trc := [
 0x0000000010300114: ret
 *)
 
-Definition bv_1 := [BV{1} 1].
-Definition bv_0 := [BV{1} 0].
-
 Definition test_state2_local (n1 : Z) Hin := {|
   seq_trace  := [];
   seq_regs   :=
     <[ "R1" := Val_Bits (BV 64 n1 Hin) ]> $
     <[ "PSTATE" := (Val_Struct
-          [("GE", Val_Poison); ("F", Val_Bits bv_1);
-          ("UAO", Val_Poison); ("C", Val_Bits bv_0);
-          ("SP", Val_Poison); ("N", Val_Bits bv_0);
-          ("Q", Val_Poison); ("A", Val_Bits bv_1); ("SS", Val_Bits bv_0);
-          ("E", Val_Poison); ("TCO", Val_Poison); ("I", Val_Bits bv_1);
-          ("PAN", Val_Poison); ("M", Val_Poison); ("D", Val_Bits bv_1);
-          ("nRW", Val_Bits bv_0); ("EL", Val_Bits bv_0);
-          ("IT", Val_Poison); ("IL", Val_Bits bv_0);
-          ("Z", Val_Bits bv_0); ("BTYPE", Val_Poison);
+          [("GE", Val_Poison); ("F", Val_Bits [BV{1} 1]);
+          ("UAO", Val_Poison); ("C", Val_Bits [BV{1} 0]);
+          ("SP", Val_Poison); ("N", Val_Bits [BV{1} 0]);
+          ("Q", Val_Poison); ("A", Val_Bits [BV{1} 1]); ("SS", Val_Bits [BV{1} 0]);
+          ("E", Val_Poison); ("TCO", Val_Poison); ("I", Val_Bits [BV{1} 1]);
+          ("PAN", Val_Poison); ("M", Val_Poison); ("D", Val_Bits [BV{1} 1]);
+          ("nRW", Val_Bits [BV{1} 0]); ("EL", Val_Bits [BV{1} 0]);
+          ("IT", Val_Poison); ("IL", Val_Bits [BV{1} 0]);
+          ("Z", Val_Bits [BV{1} 0]); ("BTYPE", Val_Poison);
           ("SSBS", Val_Poison); ("T", Val_Poison); ("J", Val_Poison);
-          ("V", Val_Bits bv_0); ("DIT", Val_Bits bv_0)]) ]> $
+          ("V", Val_Bits [BV{1} 0]); ("DIT", Val_Bits [BV{1} 0])]) ]> $
     <[ "_PC" := Val_Bits start_address ]> $
     <[ "__PC_changed" := Val_Bool false ]> $
                                              ∅;
@@ -537,11 +470,6 @@ Definition test_state2_global  := {|
 
 Definition test_state2_spec : list seq_label := [ SInstrTrap [BV{64} 0x0000000010300018] ].
 
-Lemma ite_bits b n1 n2 :
-  ite b (Val_Bits n1) (Val_Bits n2) = Val_Bits (ite b n1 n2).
-Proof. by destruct b. Qed.
-Hint Rewrite ite_bits : lithium_rewrite.
-
 Lemma test_state2_iris `{!islaG Σ} `{!threadG} n1 Hin :
   instr 0x0000000010300000 (Some [trc_cmp_x1_0]) -∗
   instr 0x0000000010300004 (Some trc_bne_0xc ) -∗
@@ -559,62 +487,24 @@ Lemma test_state2_iris `{!islaG Σ} `{!threadG} n1 Hin :
   "R0" ↦ᵣ Val_Poison -∗
   "OUT" ↦ᵣ Val_Poison -∗
   "PSTATE" ↦ᵣ (Val_Struct
-          [("GE", Val_Poison); ("F", Val_Bits bv_1);
-          ("UAO", Val_Poison); ("C", Val_Bits bv_0);
-          ("SP", Val_Poison); ("N", Val_Bits bv_0);
-          ("Q", Val_Poison); ("A", Val_Bits bv_1); ("SS", Val_Bits bv_0);
-          ("E", Val_Poison); ("TCO", Val_Poison); ("I", Val_Bits bv_1);
-          ("PAN", Val_Poison); ("M", Val_Poison); ("D", Val_Bits bv_1);
-          ("nRW", Val_Bits bv_0); ("EL", Val_Bits bv_0);
-          ("IT", Val_Poison); ("IL", Val_Bits bv_0);
-          ("Z", Val_Bits bv_0); ("BTYPE", Val_Poison);
+          [("GE", Val_Poison); ("F", Val_Bits [BV{1} 1]);
+          ("UAO", Val_Poison); ("C", Val_Bits [BV{1} 0]);
+          ("SP", Val_Poison); ("N", Val_Bits [BV{1} 0]);
+          ("Q", Val_Poison); ("A", Val_Bits [BV{1} 1]); ("SS", Val_Bits [BV{1} 0]);
+          ("E", Val_Poison); ("TCO", Val_Poison); ("I", Val_Bits [BV{1} 1]);
+          ("PAN", Val_Poison); ("M", Val_Poison); ("D", Val_Bits [BV{1} 1]);
+          ("nRW", Val_Bits [BV{1} 0]); ("EL", Val_Bits [BV{1} 0]);
+          ("IT", Val_Poison); ("IL", Val_Bits [BV{1} 0]);
+          ("Z", Val_Bits [BV{1} 0]); ("BTYPE", Val_Poison);
           ("SSBS", Val_Poison); ("T", Val_Poison); ("J", Val_Poison);
-          ("V", Val_Bits bv_0); ("DIT", Val_Bits bv_0)]) -∗
+          ("V", Val_Bits [BV{1} 0]); ("DIT", Val_Bits [BV{1} 0])]) -∗
   spec_trace test_state_spec -∗
   WPasm [].
 Proof.
   iStartProof.
-  do 100 liAStep; liShow.
-  do 100 liAStep; liShow.
-  liAStep; liShow.
-  liAStep; liShow.
-  liAStep; liShow.
-  liAStep; liShow.
-  liAStep; liShow.
-  liAStep; liShow.
-  liAStep; liShow.
-  liAStep; liShow.
-  liAStep; liShow.
-  liAStep; liShow.
-  liAStep; liShow.
-  liAStep; liShow.
-  liAStep; liShow.
-  liAStep; liShow.
-  liAStep; liShow.
-  liAStep; liShow.
-  liAStep; liShow.
-  liAStep; liShow.
-  liAStep; liShow.
-  liAStep; liShow.
-  liAStep; liShow.
-  liAStep; liShow.
+  repeat liAStep; liShow.
 
 
-
-  (* do 10 liAStep; liShow. *)
-
-
-(*
-  do 10 liAStep; liShow.
-  do 20 liAStep; liShow.
-  do 20 liAStep; liShow.
-  do 20 liAStep; liShow.
-  do 20 liAStep; liShow.
-  do 20 liAStep; liShow.
-  do 20 liAStep; liShow.
-  do 20 liAStep; liShow.
-*)
-  (* repeat liAStep; liShow. *)
 Abort.
 
 
